SyntaxMacros.v
@@ -5,63 +5,6 @@ Import ListNotations.
 Section SyntaxMacros.
   Context {pos_t method_name_t var_t reg_t: Type}.
 
-  Section ConstBits.
-    Context {fn_t: Type}.
-    Notation uaction := (uaction pos_t method_name_t var_t reg_t fn_t).
-
-    Definition UConstBits {sz} (bs: bits sz) : uaction :=
-      UConst (tau := bits_t sz) bs.
-  End ConstBits.
-
-  Context {custom_fn_t: Type}.
-  Notation uaction := (uaction pos_t method_name_t var_t reg_t (interop_ufn_t custom_fn_t)).
-
-  Definition USkip : uaction :=
-    UConstBits Ob.
-
-  Definition if_eq a1 a2 (tbranch fbranch: uaction) :=
-    UIf (UCall (UPrimFn (UConvFn UEq)) a1 a2)
-        tbranch
-        fbranch.
-
-  Fixpoint USwitch
-           (var: uaction)
-           (default: uaction)
-           (branches: list (uaction * uaction))
-    : uaction :=
-    match branches with
-    | nil => default
-    | (val, action) :: branches =>
-      if_eq var val
-            action (USwitch var default branches)
-    end.
-
-  Fixpoint gen_switch {tau}
-           (var: var_t)
-           {nb} (branches: vect (type_denote tau * uaction) (S nb)) : uaction :=
-    let '(label, branch) := vect_hd branches in
-    match nb return vect _ (S nb) -> uaction with
-    | 0 => fun _ => branch
-    | S nb => fun branches => if_eq (UVar var) (UConst label)
-                                branch (gen_switch var (vect_tl branches))
-    end branches.
-
-  Definition UCompleteSwitch
-             sz bound
-             (var: var_t)
-             (branches: vect uaction (S bound)) :=
-    gen_switch (tau := bits_t sz) var
-               (vect_map2 (fun n a => (Bits.of_nat sz (index_to_nat n), a))
-                          (all_indices (S bound)) branches).
-
-  Definition UStructInit
-             (sig: struct_sig)
-             (fields: list (string * uaction)) :=
-    let uinit := UPrimFn (UConvFn (UInit (struct_t sig))) in
-    let usubst f := UPrimFn (UStructFn (UDo SubstField f)) in
-    List.fold_left (fun acc '(f, a) => UCall (usubst f) acc a)
-                   fields (UCall uinit (UConstBits Ob) (UConstBits Ob)).
-
   Definition bits_of_ascii c : bits 8 :=
     match c with
     | Ascii.Ascii b0 b1 b2 b3 b4 b5 b6 b7 =>
@@ -74,6 +17,92 @@ Section SyntaxMacros.
     | String c s =>
       Bits.app (bits_of_bytes s) (bits_of_ascii c) (* FIXME: reversed *)
     end.
+
+  Section ConstBits.
+    Context {fn_t: Type}.
+    Notation uaction := (uaction pos_t method_name_t var_t reg_t fn_t).
+
+    Definition UConstBits {sz} (bs: bits sz) : uaction :=
+      UConst (tau := bits_t sz) bs.
+
+    Definition USkip : uaction :=
+      UConstBits Ob.
+  End ConstBits.
+
+  Section Interop.
+    Context {custom_fn_t: Type}.
+    Notation uaction := (uaction pos_t method_name_t var_t reg_t (interop_ufn_t custom_fn_t)).
+
+    Definition if_eq a1 a2 (tbranch fbranch: uaction) :=
+      UIf (UCall (UPrimFn (UConvFn UEq)) a1 a2)
+          tbranch
+          fbranch.
+
+    Fixpoint USwitch
+             (var: uaction)
+             (default: uaction)
+             (branches: list (uaction * uaction))
+      : uaction :=
+      match branches with
+      | nil => default
+      | (val, action) :: branches =>
+        if_eq var val
+              action (USwitch var default branches)
+      end.
+
+    Fixpoint gen_switch {tau}
+             (var: var_t)
+             {nb} (branches: vect (type_denote tau * uaction) (S nb)) : uaction :=
+      let '(label, branch) := vect_hd branches in
+      match nb return vect _ (S nb) -> uaction with
+      | 0 => fun _ => branch
+      | S nb => fun branches => if_eq (UVar var) (UConst label)
+                                  branch (gen_switch var (vect_tl branches))
+      end branches.
+
+    Definition UCompleteSwitch
+               sz bound
+               (var: var_t)
+               (branches: vect uaction (S bound)) :=
+      gen_switch (tau := bits_t sz) var
+                 (vect_map2 (fun n a => (Bits.of_nat sz (index_to_nat n), a))
+                            (all_indices (S bound)) branches).
+
+    Definition UStructInit
+               (sig: struct_sig)
+               (fields: list (string * uaction)) :=
+      let uinit := UPrimFn (UConvFn (UInit (struct_t sig))) in
+      let usubst f := UPrimFn (UStructFn (UDo SubstField f)) in
+      List.fold_left (fun acc '(f, a) => UCall (usubst f) acc a)
+                     fields (UCall uinit (UConstBits Ob) (UConstBits Ob)).
+  End Interop.
+
+  Section InlineCalls.
+    Context {module_reg_t: Type}.
+    Context {fn_t module_fn_t: Type}.
+    Context (fR: module_reg_t -> reg_t).
+    Context (fSigma: module_fn_t -> fn_t).
+
+    Fixpoint UCallModule (ua: uaction pos_t method_name_t var_t module_reg_t module_fn_t)
+      : uaction pos_t method_name_t var_t reg_t fn_t :=
+      match ua with
+      | UError => UError
+      | UFail tau => UFail tau
+      | UVar var => UVar var
+      | UConst cst => UConst cst
+      | UConstString s => UConstString s
+      | UConstEnum sig cst => UConstEnum sig cst
+      | UAssign v ex => UAssign v (UCallModule ex)
+      | USeq r1 r2 => USeq (UCallModule r1) (UCallModule r2)
+      | UBind v ex body => UBind v (UCallModule ex) (UCallModule body)
+      | UIf cond tbranch fbranch => UIf (UCallModule cond) (UCallModule tbranch) (UCallModule fbranch)
+      | URead port idx => URead port (fR idx)
+      | UWrite port idx value => UWrite port (fR idx) (UCallModule value)
+      | UCall fn arg1 arg2 => UCall (fSigma fn) (UCallModule arg1) (UCallModule arg2)
+      | UInternalCall sig body args => UInternalCall sig (UCallModule body) (List.map UCallModule args)
+      | UAPos p e => UAPos p (UCallModule e)
+      end.
+  End InlineCalls.
 End SyntaxMacros.
 
 Section TypedSyntaxMacros.
